books/projects/rp-rewriter/lib/mult2/meta-top.lisp
@@ -45,6 +45,8 @@
 
 (include-book "equal-meta")
 
+(include-book "adder-rules-meta")
+
 (defthm sort-sum-meta-valid-rp-meta-rulep
     (implies (and (rp-evl-meta-extract-global-facts :state state)
                   (mult-formula-checks state))
